\documentclass{beamer}
\usetheme{Boadilla}
\useoutertheme{infolines}
\setbeamertemplate{navigation symbols}{} 
\usepackage[utf8]{inputenc}
\usepackage[T1]{fontenc}
\usepackage{alphabeta}
\usepackage{graphicx}
\usepackage{mathtools}
\usepackage{amssymb}
\usepackage{amsmath}
\usepackage{amsfonts}
\usepackage[conor,links]{agda}
\usepackage{bbm}
\usepackage{newunicodechar}
\usepackage{minted}
\usepackage{xcolor}

\input{../thesis/commands}

\input{../thesis/unicode}

\title[Formal Dictionary Passing Transform]{Formal Proof of Type Preservation of the\\Dictionary Passing Transform for System F}
\institute[Uni Freiburg]{Chair of Programming Languages, University of Freiburg}
\author{Marius Weidner}


\begin{document}

\input{SystemF}
\input{SystemFo}
\input{DictionaryPassingTransform}


\begin{frame}
  \titlepage
\end{frame}

\section{Introduction}

\begin{frame}[fragile]
  \frametitle{Type Classes in Haskell}
  \begin{block}{Overloading Equality in Haskell}
    \begin{center}
      ~
      \begin{minted}[escapeinside=||]{haskell}
 class Eq α where
   eq :: α → α → Bool
 
 instance Eq Nat where
   eq x y = x ≐ y
 instance Eq α ⇒ Eq [α] where
   eq []       []       = True
   eq (x : xs) (y : ys) = eq x y && eq xs ys 
     
 .. eq 42 0 .. eq [42, 0] [42, 0] ..
      \end{minted}
      ~
    \end{center}
  \end{block}
\end{frame}

\begin{frame}[fragile]
  \frametitle{Desugaring Type Classes}
  \begin{block}{Overloading Equality in System \Fo}
    \begin{center}
      ~
      \begin{minted}[escapeinside=||]{haskell}
 |\Decl| eq in

 |\Inst| eq : Nat → Nat → Bool 
   = λx. λy. .. in
 |\Inst| eq : ∀α. [eq : α → α → Bool] ⇒ [α] → [α] → Bool 
   = Λα. ƛ(eq : α → α → Bool). λxs. λys. .. in
    
 .. eq 42 0 .. eq Nat [42, 0] [42, 0] .. 
      \end{minted}
      ~
    \end{center}
  \end{block}
\end{frame}

\begin{frame}[fragile]
  \frametitle{Dictionary Passing Transform}
  \begin{block}{Overloading Equality in System \Fo\ }
    \begin{center}
      \begin{minted}[escapeinside=||]{haskell}
 |\Decl| eq in
 |\Inst| eq : Nat → Nat → Bool 
   = λx. λy. .. in
 |\Inst| eq : ∀α. [eq : α → α → Bool] ⇒ [α] → [α] → Bool 
   = Λα. ƛ(eq : α → α → Bool). λxs. λys. .. in
 .. eq 42 0 .. eq Nat [42, 0] [42, 0] .. 
      \end{minted}
    \end{center}
  \end{block}
  \begin{block}{System \Fo\ Transformed to System F}
    \begin{center}
      \begin{minted}[escapeinside=||]{haskell}
 let eq₁ : Nat → Nat → Bool 
   = λx. λy. .. in
 let eq₂ : ∀α. (α → α → Bool) → [α] → [α] → Bool 
   = Λα. λeq₁. λxs. λys. .. in
  
 .. eq₁ 42 0 .. eq₂ Nat eq₁ [42, 0] [42, 0] .. 
      \end{minted}
    \end{center}
  \end{block}
\end{frame}

\section{Agda Formalization}

\begin{frame}[fragile]
  \frametitle{Agda Formalization of System \Fo}
  \begin{block}{Syntax Representation in Agda}
    \begin{small}
      
        \FoTerm
     
    \end{small}
  \end{block}
\end{frame}

\begin{frame}[fragile]
  \frametitle{Agda Formalization of System \Fo}
  \begin{block}{Context}
    \FoCtx
  \end{block}
  \begin{block}{Constraint Solving}
    \FoCstrSolve
  \end{block}
\end{frame}

\begin{frame}[fragile]
  \frametitle{The Dectionary Passing Transform}
\end{frame}

\section{Agda Formalization of the Dictionary Passing Transform}
\begin{frame}[fragile]
  \frametitle{Fun Lemmas on Our Way to Type Preservation}
  
\end{frame}

\begin{frame}[fragile]
  \frametitle{Type Preservation of the Dictionary Passing Transform}
  
\end{frame}


\end{document}